add more wp rules

HeapLang/State.thy
@@ -322,20 +322,8 @@ lemma head_step_to_val: "\<lbrakk>e1 \<sigma>1 \<kappa> \<Rightarrow>\<^sub>h e2
   \<Longrightarrow> \<exists>x. Some x = (to_val e2')"
   by (induction rule: head_step.induct) auto
 
-definition red :: "expr \<Rightarrow> state \<Rightarrow> bool" where
-  "red e1 \<sigma>1 \<equiv> \<exists>\<kappa> e2 \<sigma>2 efs. (e1 \<sigma>1 \<kappa> \<Rightarrow>\<^sub>h e2 \<sigma>2 efs)"
-
-lemma red_val: "red (of_val v) \<sigma> = False"
-  unfolding red_def by auto (metis option.simps(3) to_val.simps(1) val_head_stuck)
-
 lemma fill_item_not_val: "False \<longleftrightarrow> (of_val v = fill_item K e)"
   by (induction K) auto
-
-definition atomic :: "expr \<Rightarrow> bool" where
-  "atomic e \<equiv> \<forall>\<sigma>1 \<kappa> e2 \<sigma>2 efs. ((e \<sigma>1 \<kappa> \<Rightarrow>\<^sub>h e2 \<sigma>2 efs) \<longrightarrow> \<not>red e2 \<sigma>2)"
-
-definition strongly_atomic :: "expr \<Rightarrow> bool" where
-  "strongly_atomic e \<equiv> \<forall>\<sigma>1 \<kappa> e2 \<sigma>2 efs. ((e \<sigma>1 \<kappa> \<Rightarrow>\<^sub>h e2 \<sigma>2 efs) \<longrightarrow> to_val e2 \<noteq> None)"
   
 (* Other lemmata contain references to the Iris base logic and can thus not be defined yet. *)
 end
