HeapLang/LanguageDefs.thy
@@ -1,0 +1,114 @@
+theory LanguageDefs
+imports PrimitiveLaws State "../IrisCore/AuthHeap"
+begin
+
+text \<open>Auxiliary language specific definitions\<close>
+
+definition state_interp :: "state \<Rightarrow> observation list \<Rightarrow> iprop" where
+  "state_interp \<sigma> \<kappa>s = heap_interp (heap \<sigma>) \<^emph> proph_map_interp \<kappa>s (used_proph_id \<sigma>)"
+
+definition fill :: "ectx_item list \<Rightarrow> expr \<Rightarrow> expr"  where "fill K e =  fold fill_item K e"
+
+lemma fill_item_Rec: "fill_item K' e2 \<noteq> Rec f x e" by (induction K') auto
+lemma fill_Rec: "fill K e' = Rec f x e \<Longrightarrow> K =[] \<and> e' = Rec f x e"
+  apply (induction K arbitrary: e') apply (auto simp: fill_def) using fill_item_Rec by blast
+
+lemma fill_item_Val: "fill_item K e \<noteq> Val v" by (induction K) auto
+lemma fill_Val: "fill K e = Val v \<Longrightarrow> K = [] \<and> e = Val v"
+  apply (induction K arbitrary: e) apply (auto simp: fill_def) using fill_item_Val by blast
+
+datatype langCtxt = FI ectx_item | F "ectx_item list"
+fun lang_ctxt :: "langCtxt \<Rightarrow> expr \<Rightarrow> expr" where
+  "lang_ctxt (FI K) e = fill_item K e"
+| "lang_ctxt (F K) e = fill K e"
+  
+definition prim_step :: "expr \<Rightarrow> state \<Rightarrow> observation list \<Rightarrow> expr \<Rightarrow> state \<Rightarrow> expr list \<Rightarrow> bool" where
+  "prim_step e1 \<sigma>1 \<kappa> e2 \<sigma>2 efs \<equiv> \<exists>K e1' e2'. ((e1=fill K e1') \<and> (e2=fill K e2') \<and> head_step e1' \<sigma>1 \<kappa> e2' \<sigma>2 efs)"
+
+definition reducible :: "expr \<Rightarrow> state \<Rightarrow> bool" where
+  "reducible e \<sigma> \<equiv> \<exists>\<kappa> e' \<sigma>' efs. prim_step e \<sigma> \<kappa> e' \<sigma>' efs"
+
+definition reducible_no_obs :: "expr \<Rightarrow> state \<Rightarrow> bool" where
+  "reducible_no_obs e \<sigma> \<equiv> \<exists>e' \<sigma>' efs. prim_step e \<sigma> [] e' \<sigma>' efs"
+
+definition irreducible :: "expr \<Rightarrow> state \<Rightarrow> bool" where
+  "irreducible e \<sigma> \<equiv> \<forall>\<kappa> e' \<sigma>' efs. \<not>prim_step e \<sigma> \<kappa> e' \<sigma>' efs"
+
+definition stuck :: "expr \<Rightarrow> state \<Rightarrow> bool" where
+  "stuck e \<sigma> \<equiv> (to_val e = None) \<and> irreducible e \<sigma>"
+
+definition not_stuck :: "expr \<Rightarrow> state \<Rightarrow> bool" where
+  "not_stuck e \<sigma> \<equiv> (\<exists>v. to_val e = Some v) \<or> reducible e \<sigma>"
+
+lemma irred_val: "irreducible (Val v) \<sigma>"
+  unfolding irreducible_def prim_step_def
+  by (auto simp: fill_Val) (metis fill_Val option.distinct(1) to_val.simps(1) val_head_stuck)
+
+datatype stuckness = NotStuck | MaybeStuck
+instantiation stuckness :: order begin
+fun less_eq_stuckness :: "stuckness \<Rightarrow> stuckness \<Rightarrow> bool" where
+  "less_eq_stuckness MaybeStuck NotStuck = False"
+| "less_eq_stuckness _ _ = True"
+fun less_stuckness :: "stuckness \<Rightarrow> stuckness \<Rightarrow> bool" where
+  "less_stuckness MaybeStuck NotStuck = False"
+| "less_stuckness MaybeStuck MaybeStuck = False"
+| "less_stuckness NotStuck NotStuck = False"
+| "less_stuckness _ _ = True"
+instance proof
+  fix x y :: stuckness
+  show "(x < y) = (x \<le> y \<and> \<not> y \<le> x)" by (cases x; cases y) auto
+next
+  fix x :: stuckness
+  show "x\<le>x" by (cases x) auto
+next
+  fix x y z :: stuckness
+  show "x \<le> y \<Longrightarrow> y \<le> z \<Longrightarrow> x \<le> z" by (cases x; cases y; cases z) auto
+next
+  fix x y :: stuckness
+  show "x \<le> y \<Longrightarrow> y \<le> x \<Longrightarrow> x = y" by (cases x; cases y) auto
+qed
+end
+
+datatype atomicity = StronglyAtomic | WeaklyAtomic
+
+definition stuckness_to_atomicity :: "stuckness \<Rightarrow> atomicity" where
+  "stuckness_to_atomicity s = (case s of MaybeStuck \<Rightarrow> StronglyAtomic | NotStuck \<Rightarrow> WeaklyAtomic)"
+
+definition atomic :: "atomicity \<Rightarrow> expr \<Rightarrow> bool" where
+  "atomic a e \<equiv> \<forall>\<sigma> e' \<kappa> \<sigma>' efs. prim_step e \<sigma> \<kappa> e' \<sigma>' efs \<longrightarrow> 
+    (case a of WeaklyAtomic \<Rightarrow> irreducible e' \<sigma>' | StronglyAtomic \<Rightarrow> (\<exists>v. to_val e' = Some v))"
+
+text \<open>Atomicity proofs, but mostly axiomatized.\<close>
+    
+lemma atomic_rec: "atomic a (Rec f x e)" 
+proof (auto simp: atomic_def prim_step_def)
+  fix \<sigma> \<kappa> \<sigma>' efs K e1' e2'
+  assume assms: "Rec f x e = fill K e1'" "e1' \<sigma> \<kappa> \<Rightarrow>\<^sub>h e2' \<sigma>' efs"
+  from fill_Rec[OF assms(1)[symmetric]] have K: "K = []" "e1' = Rec f x e" by simp_all
+  with assms(2) have "\<kappa>=[]" "e2' = Val(RecV f x e)" "efs = []" by auto
+  with K have "fill K e2' = Val(RecV f x e)" unfolding fill_def by simp
+  then show "case a of StronglyAtomic \<Rightarrow> \<exists>v. to_val (fill K e2') = Some v | WeaklyAtomic \<Rightarrow> irreducible (fill K e2') \<sigma>'"
+  by (cases a) (auto simp: irred_val)
+qed
+
+lemma atomic_pair: "atomic a (Pair (Val v1) (Val v2))" sorry
+lemma atomic_injl: "atomic a (InjL (Val v))" sorry
+lemma atomic_injr: "atomic a (InjR (Val v))" sorry
+lemma atomic_beta: "atomic a (App (RecV f x (Val v1)) (Val v2))" sorry
+lemma atomic_unop: "atomic a (UnOp uop (Val v))" sorry
+lemma atomic_binop: "atomic a (BinOp bop (Val v1) (Val v2))" sorry
+lemma atomic_if_true: "atomic a (If (Val (LitV (LitBool True))) (Val v1) e2)" sorry
+lemma atomic_if_false: "atomic a (If (Val (LitV (LitBool False))) e1 (Val v2))" sorry
+lemma atomic_fst: "atomic a (Fst (Val v))" sorry
+lemma atomic_snd: "atomic a (Snd (Val v))" sorry
+lemma atomic_fork: "atomic a (Fork e)" sorry
+lemma atomic_alloc: "atomic a (AllocN (Val v1) (Val v2))" sorry
+lemma atomic_free: "atomic a (Free (Val v))" sorry
+lemma atomic_load: "atomic a (Load (Val v))" sorry
+lemma atomic_xchg: "atomic a (Xchg (Val v1) (Val v2))" sorry
+lemma atomic_store: "atomic a (Store (Val v1) (Val v2))" sorry
+lemma atomic_cmp_xchg: "atomic a (CmpXchg (Val v0) (Val v1) (Val v2))" sorry
+lemma atomic_faa: "atomic a (FAA (Val v1) (Val v2))" sorry
+lemma atomic_new_proph: "atomic a NewProph" sorry
+lemma atomic_resolve: "atomic a e \<Longrightarrow> atomic a (Resolve e (Val v1) (Val v2))" sorry
+end
